code/bignum/Hacl.GenericField32.fsti
@@ -121,7 +121,7 @@ val one: len:Ghost.erased _ -> MA.bn_field_one_st t_limbs len
 
   Before calling this function, the caller will need to ensure that the following
   preconditions are observed.
-  • 0 < b
+  • 0 < bBits
   • b < pow2 bBits "]
 val exp_consttime: len:Ghost.erased _ -> MA.bn_field_exp_consttime_st t_limbs len
 
@@ -140,7 +140,7 @@ val exp_consttime: len:Ghost.erased _ -> MA.bn_field_exp_consttime_st t_limbs le
 
   Before calling this function, the caller will need to ensure that the following
   preconditions are observed.
-  • 0 < b
+  • 0 < bBits
   • b < pow2 bBits "]
 val exp_vartime: len:Ghost.erased _ -> MA.bn_field_exp_vartime_st t_limbs len
 
